Test/civl/async/tds.bpl
@@ -1,8 +1,6 @@
 // RUN: %parallel-boogie "%s" > "%t"
 // RUN: %diff "%s.expect" "%t"
 
-type {:linear "tid"} Tid = int;
-
 const unique DEFAULT: int;
 const unique CREATED: int;
 const unique PROCESSED: int;
@@ -10,36 +8,36 @@ const unique FINISHED: int;
 
 var status:[int]int;
 
-atomic action {:layer 5} atomic_main({:linear "tid"} id: int, {:linear_in "tid"} tids: [int]bool)
+atomic action {:layer 5} atomic_main({:linear} id: One int, {:linear_in} tids: Set int)
 modifies status;
 {
-    assert id == c;
-    assert (forall i: int :: (0 <= i && i < n) <==> tids[i]);
+    assert id->val == c;
+    assert (forall i: int :: (0 <= i && i < n) <==> Set_Contains(tids, i));
     assert (forall i: int :: 0 <= i && i < n ==> status[i] == DEFAULT);
     status := (lambda j: int :: if (0 <= j && j < n) then FINISHED else status[j]);
 }
 
-left action {:layer 4} atomic_server({:linear "tid"} id: int, {:linear_in "tid"} tids: [int]bool)
+left action {:layer 4} atomic_server({:linear} id: One int, {:linear_in} tids: Set int)
 modifies status;
 {
-    assert id == c;
-    assert (forall i: int :: (0 <= i && i < n) <==> tids[i]);
+    assert id->val == c;
+    assert (forall i: int :: (0 <= i && i < n) <==> Set_Contains(tids, i));
     assert (forall i: int :: 0 <= i && i < n ==> status[i] == DEFAULT);
     status := (lambda j: int :: if (0 <= j && j < n) then CREATED else status[j]);
 }
 
-left action {:layer 4} atomic_client({:linear "tid"} id: int)
+left action {:layer 4} atomic_client({:linear} id: One int)
 modifies status;
 {
-    assert id == c;
+    assert id->val == c;
     assert (forall i: int :: 0 <= i && i < n ==> status[i] == CREATED);
     status := (lambda j: int :: if (0 <= j && j < n) then PROCESSED else status[j]);
 }
 
-left action {:layer 4} atomic_master({:linear "tid"} id: int)
+left action {:layer 4} atomic_master({:linear} id: One int)
 modifies status;
 {
-    assert id == c;
+    assert id->val == c;
     assert (forall i: int :: 0 <= i && i < n ==> status[i] == PROCESSED);
     status := (lambda j: int :: if (0 <= j && j < n) then FINISHED else status[j]);
 }
@@ -48,7 +46,7 @@ const c: int;
 const n: int;
 axiom 0 <= n;
 
-yield procedure {:layer 4} main({:linear "tid"} id: int, {:linear_in "tid"} tids: [int]bool)
+yield procedure {:layer 4} main({:linear} id: One int, {:linear_in} tids: Set int)
 refines atomic_main;
 {
     var i: int;
@@ -61,25 +59,25 @@ refines atomic_main;
     call master3(id);
 }
 
-yield procedure {:layer 2} Alloc(i: int, {:linear_in "tid"} tidq: [int]bool) returns ({:linear "tid"} id: int, {:linear "tid"} tidq':[int]bool);
+yield procedure {:layer 2} Alloc(i: int, {:linear_in} tidq: Set int) returns ({:linear} id: One int, {:linear} tidq': Set int);
 refines AtomicAlloc;
-both action {:layer 3} AtomicAlloc(i: int, {:linear_in "tid"} tidq: [int]bool) returns ({:linear "tid"} id: int, {:linear "tid"} tidq':[int]bool)
-{ assert tidq[i]; id := i; tidq' := tidq[i := false]; }
+both action {:layer 3} AtomicAlloc(i: int, {:linear_in} tidq: Set int) returns ({:linear} id: One int, {:linear} tidq': Set int)
+{ id := One(i); tidq' := tidq; call One_Split(tidq', id); }
 
-yield procedure {:layer 3} server3({:linear "tid"} id: int, {:linear_in "tid"} tids: [int]bool)
+yield procedure {:layer 3} server3({:linear} id: One int, {:linear_in} tids: Set int)
 refines atomic_server;
 {
     var i: int;
     var {:layer 3} snapshot: [int]int;
-    var {:linear "tid"} tids': [int]bool;
-    var {:linear "tid"} tid: int;
+    var {:linear} tids': Set int;
+    var {:linear} tid: One int;
 
     i := 0;
     call {:layer 3} snapshot := Copy(status);
     tids' := tids;
     while (i < n)
     invariant {:layer 3} 0 <= i && i <= n;
-    invariant {:layer 3} (forall j: int :: i <= j && j < n <==> tids'[j]);
+    invariant {:layer 3} (forall j: int :: i <= j && j < n <==> Set_Contains(tids', j));
     invariant {:layer 3} status == (lambda j: int :: if (0 <= j && j < i) then CREATED else snapshot[j]);
     {
         call tid, tids' := Alloc(i, tids');
@@ -88,16 +86,16 @@ refines atomic_server;
     }
 }
 
-left action {:layer 3} atomic_server2({:linear "tid"} i: int)
+left action {:layer 3} atomic_server2({:linear} i: One int)
 modifies status;
 {
-    assert status[i] == DEFAULT;
-    status[i] := CREATED;
+    assert status[i->val] == DEFAULT;
+    status[i->val] := CREATED;
 }
-yield procedure {:layer 2} server2({:linear "tid"} i: int);
+yield procedure {:layer 2} server2({:linear} i: One int);
 refines atomic_server2;
 
-yield procedure {:layer 3} client3({:linear "tid"} id: int)
+yield procedure {:layer 3} client3({:linear} id: One int)
 refines atomic_client;
 {
     call client2();
@@ -112,7 +110,7 @@ modifies status;
 yield procedure {:layer 2} client2();
 refines atomic_client2;
 
-yield procedure {:layer 3} master3({:linear "tid"} id: int)
+yield procedure {:layer 3} master3({:linear} id: One int)
 refines atomic_master;
 {
     call master2();
