Test/civl/regression-tests/linearity-bug-1.bpl
@@ -2,7 +2,7 @@
 // RUN: %diff "%s.expect" "%t"
 
 var {:layer 0,1} n : int;
-var {:linear "tid"} {:layer 0,1} S : TidSet;
+var {:linear} {:layer 0,1} S : Set int;
 
 // This test exposed a bug in the commutativity checker. Since t is linear_in,
 // it does not have to be available after the atomic action executed. However,
@@ -10,11 +10,11 @@ var {:linear "tid"} {:layer 0,1} S : TidSet;
 // commutativity checker procedure contained t and thus made the whole
 // postcondition 'vacuously' (because t is added to A) true.
 
-atomic action {:layer 1} atomic_inc_n ({:linear_in "tid"} t : Tid)
+atomic action {:layer 1} atomic_inc_n ({:linear_in} t : One int)
 modifies S, n;
-{ assert !S[t]; S[t] := true; n := n + 1; }
+{ call One_Put(S, t); n := n + 1; }
 
-yield procedure {:layer 0} inc_n ({:linear_in "tid"} t : Tid);
+yield procedure {:layer 0} inc_n ({:linear_in} t : One int);
 refines atomic_inc_n;
 
 right action {:layer 1} atomic_read_n () returns (ret : int)
@@ -22,6 +22,3 @@ right action {:layer 1} atomic_read_n () returns (ret : int)
 
 yield procedure {:layer 0} read_n () returns (ret : int);
 refines atomic_read_n;
-
-type {:linear "tid"} Tid = int;
-type TidSet = [Tid]bool;
