Test/civl/regression-tests/linear/f3.bpl
@@ -1,10 +1,9 @@
 // RUN: %parallel-boogie "%s" > "%t"
 // RUN: %diff "%s.expect" "%t"
-type {:linear "tid"} X = int;
 
 procedure A() {}
 
-procedure B({:linear_in "tid"} tid:int) returns({:linear "tid"} tid':int)
+procedure B({:linear_in} tid:int) returns({:linear} tid':int)
 {
   tid' := tid;
   call A();
