Test/civl/regression-tests/permissions.bpl
@@ -1,0 +1,39 @@
+// RUN: %parallel-boogie "%s" > "%t"
+// RUN: %diff "%s.expect" "%t"
+
+yield procedure {:layer 1} Proc0 ({:linear} x: One int, {:linear} y: One int)
+{
+  assert {:layer 1} x != y;
+}
+
+var {:linear} {:layer 0,1} A : Set int;
+
+yield procedure {:layer 1} Proc1 ({:linear} i: One int)
+{
+  call {:layer 1} Lemma(A, i);
+}
+
+pure procedure Lemma (set: Set int, i: One int);
+requires !Set_Contains(set, i->val);
+
+datatype D { D1({:linear} x: One int), D2({:linear} x: One int) }
+
+yield procedure {:layer 1} Proc2 ({:linear} d: D)
+{
+  call {:layer 1} Lemma(A, d->x);
+}
+
+datatype E { E({:linear} d: D) }
+
+yield procedure {:layer 1} Proc3 ({:linear} e: E)
+{
+  call {:layer 1} Lemma(A, e->d->x);
+}
+
+datatype D' { X({:linear} x: One int), Y(x: One int) }
+
+yield procedure {:layer 1} Proc4 ({:linear} d: D')
+requires {:layer 1} d is X;
+{
+  call {:layer 1} Lemma(A, d->x);
+}
